Examples/ERC20/Correct.lean
@@ -6,7 +6,7 @@ import Examples.ERC20.Allowance
 import Examples.ERC20.Approve
 import Examples.ERC20.Transfer
 import Examples.ERC20.TransferFrom
-import Reasoning.ABIDecode
+import Reasoning.ABI
 import Reasoning.Theory
 import Reasoning.Stepping
 import Reasoning.Reach
